Clean up select

Superposition_Calculus/First_Order_Superposition.thy
@@ -3,10 +3,11 @@ theory First_Order_Superposition
     Nonground_Order
     Saturation_Framework.Lifting_to_Non_Ground_Calculi
     Ground_Superposition
-    First_Order_Select
+    Nonground_Selection_Function
     Renaming
     Nonground_Typing
 begin
+
 
 hide_type Inference_System.inference
 hide_const
@@ -15,7 +16,6 @@ hide_const
   Inference_System.concl_of
   Inference_System.main_prem_of
 
-(* TODO: Remove Restricted_Predicates all together? *)
 (* Hide as much of Restricted_Predicates.wfp_on as possible *)
 hide_fact
   Restricted_Predicates.wfp_on_imp_minimal
@@ -42,139 +42,129 @@ hide_fact
 
 section \<open>First-Order Layer\<close>
 
-
 locale first_order_superposition_calculus =
-  test +
-  nonground_typing typeof_fun +
+  nonground_typing \<F> +
   nonground_order less\<^sub>t +
-  first_order_select select
+  nonground_selection_function select
   for
-    select :: "('f, ('v :: infinite)) select" and
+    select :: "('f, 'v :: infinite) select" and
     less\<^sub>t :: "('f, 'v) term \<Rightarrow> ('f, 'v) term \<Rightarrow> bool" and
-    typeof_fun :: "('f, 'ty) fun_types" + (* TODO: rename to \<F> *)
+    \<F> :: "('f, 'ty) fun_types" +
   fixes
-    tiebreakers :: "'f gatom clause  \<Rightarrow> ('f, 'v) atom clause \<Rightarrow> ('f, 'v) atom clause \<Rightarrow> bool" 
+    tiebreakers :: "'f gatom clause \<Rightarrow> ('f, 'v) atom clause \<Rightarrow> ('f, 'v) atom clause \<Rightarrow> bool" 
   assumes
-    wellfounded_tiebreakers: 
-      "\<And>clause\<^sub>G. wfP (tiebreakers clause\<^sub>G) \<and> 
-               transp (tiebreakers clause\<^sub>G) \<and> 
-               asymp (tiebreakers clause\<^sub>G)" and
+    tiebreakers: "\<And>C\<^sub>G. wellfounded_strict_order (tiebreakers C\<^sub>G)" and
   (* TODO/ Note: Was not needed without types \<rightarrow> Discuss *)
-    function_symbols: "\<And>\<tau>. \<exists>f. typeof_fun f = ([], \<tau>)" and
-    ground_critical_pair_theorem: "\<And>(R :: 'f gterm rel). ground_critical_pair_theorem R" and
-    variables: "|UNIV :: 'ty set| \<le>o |UNIV :: 'v set|"
+    function_symbols: "\<And>\<tau>. \<exists>f. \<F> f = ([], \<tau>)" and
+    variables: "|UNIV :: 'ty set| \<le>o |UNIV :: 'v set|" and
+    ground_critical_pair_theorem: "\<And>(R :: 'f gterm rel). ground_critical_pair_theorem R"
 begin
 
 interpretation term_order_notation.
 
+sublocale tiebreakers: wellfounded_strict_order "tiebreakers C\<^sub>G"
+  by (rule tiebreakers)
+
 abbreviation typed_tiebreakers :: 
-      "'f gatom clause \<Rightarrow> ('f, 'v, 'ty) typed_clause \<Rightarrow> ('f, 'v, 'ty) typed_clause \<Rightarrow> bool" where 
-    "typed_tiebreakers clause\<^sub>G clause\<^sub>1 clause\<^sub>2 \<equiv> tiebreakers clause\<^sub>G (fst clause\<^sub>1) (fst clause\<^sub>2)"
+  "'f gatom clause \<Rightarrow> ('f, 'v, 'ty) typed_clause \<Rightarrow> ('f, 'v, 'ty) typed_clause \<Rightarrow> bool" where 
+  "typed_tiebreakers C\<^sub>G C\<^sub>1 C\<^sub>2 \<equiv> tiebreakers C\<^sub>G (fst C\<^sub>1) (fst C\<^sub>2)"
 
-lemma wellfounded_typed_tiebreakers: 
-      "wfP (typed_tiebreakers clause\<^sub>G) \<and> 
-       transp (typed_tiebreakers clause\<^sub>G) \<and>
-      asymp (typed_tiebreakers clause\<^sub>G)"
-proof(intro conjI)
+sublocale typed_tiebreakers: wellfounded_strict_order "typed_tiebreakers C\<^sub>G"
+proof unfold_locales
+  show "transp (typed_tiebreakers C\<^sub>G)"
+    using tiebreakers.transp 
+    unfolding transp_def 
+    by blast
 
-  show "wfp (typed_tiebreakers clause\<^sub>G)"
-    using wellfounded_tiebreakers
-    by (meson wfp_if_convertible_to_wfp)
-
-  show "transp (typed_tiebreakers clause\<^sub>G)"
-    using wellfounded_tiebreakers
-    by (smt (verit, ccfv_threshold) transpD transpI)
-
-  show "asymp (typed_tiebreakers clause\<^sub>G)"
-    using wellfounded_tiebreakers
+  show "asymp (typed_tiebreakers C\<^sub>G)"
+    using tiebreakers.asymp
     by (meson asympD asympI)
-qed
 
-definition is_merged_var_type_env where
-  "is_merged_var_type_env \<V> X \<V>\<^sub>X \<rho>\<^sub>X Y \<V>\<^sub>Y \<rho>\<^sub>Y \<equiv>
-    (\<forall>x \<in> X. welltyped \<V> (\<rho>\<^sub>X x) (\<V>\<^sub>X x)) \<and>
-    (\<forall>y \<in> Y. welltyped \<V> (\<rho>\<^sub>Y y) (\<V>\<^sub>Y y))"
+  show "wfp (typed_tiebreakers C\<^sub>G)"
+    using tiebreakers.wfp
+    by (meson wfp_if_convertible_to_wfp)
+qed
 
 inductive eq_resolution :: "('f, 'v, 'ty) typed_clause \<Rightarrow> ('f, 'v, 'ty) typed_clause \<Rightarrow> bool" where
   eq_resolutionI: 
-   "premise = add_mset literal premise' \<Longrightarrow>
-    literal = term !\<approx> term' \<Longrightarrow>
-    term_subst.is_imgu \<mu> {{ term, term' }} \<Longrightarrow>
-    welltyped_imgu \<V> term term' \<mu> \<Longrightarrow>
-    select premise = {#} \<and> is_maximal (literal \<cdot>l \<mu>) (premise \<cdot> \<mu>) \<or> 
-      is_maximal (literal \<cdot>l \<mu>) ((select premise) \<cdot> \<mu>) \<Longrightarrow>
-    conclusion = premise' \<cdot> \<mu> \<Longrightarrow>
-    eq_resolution (premise, \<V>) (conclusion, \<V>)"
+   "D = add_mset l D' \<Longrightarrow>
+    l = t !\<approx> t' \<Longrightarrow>
+    term.is_imgu \<mu> {{ t, t' }} \<Longrightarrow>
+    welltyped_imgu \<V> t t' \<mu> \<Longrightarrow>
+    select D = {#} \<and> is_maximal (l \<cdot>l \<mu>) (D \<cdot> \<mu>) \<or> is_maximal (l \<cdot>l \<mu>) (select D \<cdot> \<mu>) \<Longrightarrow>
+    C = D' \<cdot> \<mu> \<Longrightarrow>
+    eq_resolution (D, \<V>) (C, \<V>)"
 
 inductive eq_factoring :: "('f, 'v, 'ty) typed_clause \<Rightarrow> ('f, 'v, 'ty) typed_clause \<Rightarrow> bool" where
   eq_factoringI: "
-    premise = add_mset literal\<^sub>1 (add_mset literal\<^sub>2 premise') \<Longrightarrow>
-    literal\<^sub>1 = term\<^sub>1 \<approx> term\<^sub>1' \<Longrightarrow>
-    literal\<^sub>2 = term\<^sub>2 \<approx> term\<^sub>2' \<Longrightarrow>
-    select premise = {#} \<Longrightarrow> 
-    is_maximal (literal\<^sub>1 \<cdot>l \<mu>) (premise \<cdot> \<mu>) \<Longrightarrow>
-    \<not> (term\<^sub>1 \<cdot>t \<mu> \<preceq>\<^sub>t term\<^sub>1' \<cdot>t \<mu>) \<Longrightarrow>
-    term_subst.is_imgu \<mu> {{ term\<^sub>1, term\<^sub>2 }} \<Longrightarrow>
-    welltyped_imgu \<V> term\<^sub>1 term\<^sub>2 \<mu> \<Longrightarrow>
-    conclusion = add_mset (term\<^sub>1 \<approx> term\<^sub>2') (add_mset (term\<^sub>1' !\<approx> term\<^sub>2') premise') \<cdot> \<mu> \<Longrightarrow>
-    eq_factoring (premise, \<V>) (conclusion, \<V>)"
+    D = add_mset l\<^sub>1 (add_mset l\<^sub>2 D') \<Longrightarrow>
+    l\<^sub>1 = t\<^sub>1 \<approx> t\<^sub>1' \<Longrightarrow>
+    l\<^sub>2 = t\<^sub>2 \<approx> t\<^sub>2' \<Longrightarrow>
+    select D = {#} \<Longrightarrow> 
+    is_maximal (l\<^sub>1 \<cdot>l \<mu>) (D \<cdot> \<mu>) \<Longrightarrow>
+    \<not> (t\<^sub>1 \<cdot>t \<mu> \<preceq>\<^sub>t t\<^sub>1' \<cdot>t \<mu>) \<Longrightarrow>
+    term.is_imgu \<mu> {{ t\<^sub>1, t\<^sub>2 }} \<Longrightarrow>
+    welltyped_imgu \<V> t\<^sub>1 t\<^sub>2 \<mu> \<Longrightarrow>
+    C = add_mset (t\<^sub>1 \<approx> t\<^sub>2') (add_mset (t\<^sub>1' !\<approx> t\<^sub>2') D') \<cdot> \<mu> \<Longrightarrow>
+    eq_factoring (D, \<V>) (C, \<V>)"
 
 (* TODO: Not sure if welltypedness for renaming is necessary, I think it's already implied *)
 (* TODO: welltyped_on for imgu *)
-(* TODO: weaken  all_types \<V>\<^sub>1 \<Longrightarrow> all_types \<V>\<^sub>2 *)
+(* TODO: weaken  infinite_variables_per_type \<V>\<^sub>1 \<Longrightarrow> infinite_variables_per_type \<V>\<^sub>2 *)
+(* TODO: Order of conditions *)
+(* TODO: Get things like is_renaming out of the name scope *)
+(* TODO: \<P> \<in> {Pos, Neg} *)
 inductive superposition ::
   "('f, 'v, 'ty) typed_clause \<Rightarrow> ('f, 'v, 'ty) typed_clause \<Rightarrow> ('f, 'v, 'ty) typed_clause \<Rightarrow> bool"
 where
   superpositionI:
-   "term_subst.is_renaming \<rho>\<^sub>1 \<Longrightarrow>
-    term_subst.is_renaming \<rho>\<^sub>2 \<Longrightarrow>
-    clause.vars (premise\<^sub>1 \<cdot> \<rho>\<^sub>1) \<inter>  clause.vars (premise\<^sub>2 \<cdot> \<rho>\<^sub>2) = {} \<Longrightarrow>
-    premise\<^sub>1 = add_mset literal\<^sub>1 premise\<^sub>1' \<Longrightarrow>
-    premise\<^sub>2 = add_mset literal\<^sub>2 premise\<^sub>2' \<Longrightarrow>
+   "term.is_renaming \<rho>\<^sub>1 \<Longrightarrow>
+    term.is_renaming \<rho>\<^sub>2 \<Longrightarrow>
+    clause.vars (E \<cdot> \<rho>\<^sub>1) \<inter>  clause.vars (D \<cdot> \<rho>\<^sub>2) = {} \<Longrightarrow>
+    E = add_mset l\<^sub>1 E' \<Longrightarrow>
+    D = add_mset l\<^sub>2 D' \<Longrightarrow>
     \<P> \<in> {Pos, Neg} \<Longrightarrow>
-    literal\<^sub>1 = \<P> (Upair context\<^sub>1\<langle>term\<^sub>1\<rangle> term\<^sub>1') \<Longrightarrow>
-    literal\<^sub>2 = term\<^sub>2 \<approx> term\<^sub>2' \<Longrightarrow>
-    \<not> is_Var term\<^sub>1 \<Longrightarrow>
-    term_subst.is_imgu \<mu> {{term\<^sub>1 \<cdot>t \<rho>\<^sub>1, term\<^sub>2 \<cdot>t \<rho>\<^sub>2}} \<Longrightarrow>
-    welltyped_imgu \<V>\<^sub>3 (term\<^sub>1 \<cdot>t \<rho>\<^sub>1) (term\<^sub>2 \<cdot>t \<rho>\<^sub>2) \<mu> \<Longrightarrow>
-    \<forall>x \<in> clause.vars (premise\<^sub>1 \<cdot> \<rho>\<^sub>1). \<V>\<^sub>1 (inv \<rho>\<^sub>1 (Var x)) = \<V>\<^sub>3 x \<Longrightarrow>
-    \<forall>x \<in> clause.vars (premise\<^sub>2 \<cdot> \<rho>\<^sub>2). \<V>\<^sub>2 (inv \<rho>\<^sub>2 (Var x)) = \<V>\<^sub>3 x \<Longrightarrow>
-    is_welltyped_on (clause.vars premise\<^sub>1) \<V>\<^sub>1 \<rho>\<^sub>1 \<Longrightarrow>
-    is_welltyped_on (clause.vars premise\<^sub>2) \<V>\<^sub>2 \<rho>\<^sub>2 \<Longrightarrow>
-    (\<And>\<tau> \<tau>'. typed \<V>\<^sub>2 term\<^sub>2 \<tau> \<Longrightarrow> typed \<V>\<^sub>2 term\<^sub>2' \<tau>' \<Longrightarrow> \<tau> = \<tau>') \<Longrightarrow>
-    \<not> (premise\<^sub>1 \<cdot> \<rho>\<^sub>1 \<cdot> \<mu> \<preceq>\<^sub>c premise\<^sub>2 \<cdot> \<rho>\<^sub>2 \<cdot> \<mu>) \<Longrightarrow>
+    l\<^sub>1 = \<P> (Upair c\<^sub>1\<langle>t\<^sub>1\<rangle> t\<^sub>1') \<Longrightarrow>
+    l\<^sub>2 = t\<^sub>2 \<approx> t\<^sub>2' \<Longrightarrow>
+    \<not> is_Var t\<^sub>1 \<Longrightarrow>
+    term.is_imgu \<mu> {{t\<^sub>1 \<cdot>t \<rho>\<^sub>1, t\<^sub>2 \<cdot>t \<rho>\<^sub>2}} \<Longrightarrow>
+    welltyped_imgu \<V>\<^sub>3 (t\<^sub>1 \<cdot>t \<rho>\<^sub>1) (t\<^sub>2 \<cdot>t \<rho>\<^sub>2) \<mu> \<Longrightarrow>
+    \<forall>x \<in> clause.vars (E \<cdot> \<rho>\<^sub>1). \<V>\<^sub>1 (inv \<rho>\<^sub>1 (Var x)) = \<V>\<^sub>3 x \<Longrightarrow>
+    \<forall>x \<in> clause.vars (D \<cdot> \<rho>\<^sub>2). \<V>\<^sub>2 (inv \<rho>\<^sub>2 (Var x)) = \<V>\<^sub>3 x \<Longrightarrow>
+    is_welltyped_on (clause.vars E) \<V>\<^sub>1 \<rho>\<^sub>1 \<Longrightarrow>
+    is_welltyped_on (clause.vars D) \<V>\<^sub>2 \<rho>\<^sub>2 \<Longrightarrow>
+    (\<And>\<tau> \<tau>'. typed \<V>\<^sub>2 t\<^sub>2 \<tau> \<Longrightarrow> typed \<V>\<^sub>2 t\<^sub>2' \<tau>' \<Longrightarrow> \<tau> = \<tau>') \<Longrightarrow>
+    \<not> (E \<cdot> \<rho>\<^sub>1 \<cdot> \<mu> \<preceq>\<^sub>c D \<cdot> \<rho>\<^sub>2 \<cdot> \<mu>) \<Longrightarrow>
     (\<P> = Pos 
-      \<and> select premise\<^sub>1 = {#} 
-      \<and> is_strictly_maximal (literal\<^sub>1 \<cdot>l \<rho>\<^sub>1 \<cdot>l \<mu>) (premise\<^sub>1 \<cdot> \<rho>\<^sub>1 \<cdot> \<mu>)) \<or>
+      \<and> select E = {#} 
+      \<and> is_strictly_maximal (l\<^sub>1 \<cdot>l \<rho>\<^sub>1 \<cdot>l \<mu>) (E \<cdot> \<rho>\<^sub>1 \<cdot> \<mu>)) \<or>
     (\<P> = Neg 
-      \<and> (select premise\<^sub>1 = {#} \<and> is_maximal (literal\<^sub>1 \<cdot>l \<rho>\<^sub>1 \<cdot>l \<mu>) (premise\<^sub>1 \<cdot> \<rho>\<^sub>1 \<cdot> \<mu>) 
-          \<or> is_maximal (literal\<^sub>1 \<cdot>l \<rho>\<^sub>1 \<cdot>l \<mu>) ((select premise\<^sub>1) \<cdot> \<rho>\<^sub>1 \<cdot> \<mu>))) \<Longrightarrow>
-    select premise\<^sub>2 = {#} \<Longrightarrow>
-    is_strictly_maximal (literal\<^sub>2 \<cdot>l \<rho>\<^sub>2 \<cdot>l \<mu>) (premise\<^sub>2 \<cdot> \<rho>\<^sub>2 \<cdot> \<mu>) \<Longrightarrow>
-    \<not> (context\<^sub>1\<langle>term\<^sub>1\<rangle> \<cdot>t \<rho>\<^sub>1 \<cdot>t \<mu> \<preceq>\<^sub>t term\<^sub>1' \<cdot>t \<rho>\<^sub>1 \<cdot>t \<mu>) \<Longrightarrow>
-    \<not> (term\<^sub>2 \<cdot>t \<rho>\<^sub>2 \<cdot>t \<mu> \<preceq>\<^sub>t term\<^sub>2' \<cdot>t \<rho>\<^sub>2 \<cdot>t \<mu>) \<Longrightarrow>
-    conclusion = add_mset (\<P> (Upair (context\<^sub>1 \<cdot>t\<^sub>c \<rho>\<^sub>1)\<langle>term\<^sub>2' \<cdot>t \<rho>\<^sub>2\<rangle> (term\<^sub>1' \<cdot>t \<rho>\<^sub>1))) 
-          (premise\<^sub>1' \<cdot> \<rho>\<^sub>1 + premise\<^sub>2' \<cdot> \<rho>\<^sub>2) \<cdot> \<mu> \<Longrightarrow>
-    all_types \<V>\<^sub>1 \<Longrightarrow> all_types \<V>\<^sub>2 \<Longrightarrow>
-    superposition (premise\<^sub>2, \<V>\<^sub>2) (premise\<^sub>1, \<V>\<^sub>1) (conclusion, \<V>\<^sub>3)"
+      \<and> (select E = {#} \<and> is_maximal (l\<^sub>1 \<cdot>l \<rho>\<^sub>1 \<cdot>l \<mu>) (E \<cdot> \<rho>\<^sub>1 \<cdot> \<mu>) 
+          \<or> is_maximal (l\<^sub>1 \<cdot>l \<rho>\<^sub>1 \<cdot>l \<mu>) ((select E) \<cdot> \<rho>\<^sub>1 \<cdot> \<mu>))) \<Longrightarrow>
+    select D = {#} \<Longrightarrow>
+    is_strictly_maximal (l\<^sub>2 \<cdot>l \<rho>\<^sub>2 \<cdot>l \<mu>) (D \<cdot> \<rho>\<^sub>2 \<cdot> \<mu>) \<Longrightarrow>
+    \<not> (c\<^sub>1\<langle>t\<^sub>1\<rangle> \<cdot>t \<rho>\<^sub>1 \<cdot>t \<mu> \<preceq>\<^sub>t t\<^sub>1' \<cdot>t \<rho>\<^sub>1 \<cdot>t \<mu>) \<Longrightarrow>
+    \<not> (t\<^sub>2 \<cdot>t \<rho>\<^sub>2 \<cdot>t \<mu> \<preceq>\<^sub>t t\<^sub>2' \<cdot>t \<rho>\<^sub>2 \<cdot>t \<mu>) \<Longrightarrow>
+    C = add_mset (\<P> (Upair (c\<^sub>1 \<cdot>t\<^sub>c \<rho>\<^sub>1)\<langle>t\<^sub>2' \<cdot>t \<rho>\<^sub>2\<rangle> (t\<^sub>1' \<cdot>t \<rho>\<^sub>1))) (E' \<cdot> \<rho>\<^sub>1 + D' \<cdot> \<rho>\<^sub>2) \<cdot> \<mu> \<Longrightarrow>
+    infinite_variables_per_type \<V>\<^sub>1 \<Longrightarrow> 
+    infinite_variables_per_type \<V>\<^sub>2 \<Longrightarrow>
+    superposition (D, \<V>\<^sub>2) (E, \<V>\<^sub>1) (C, \<V>\<^sub>3)"
 
 abbreviation eq_factoring_inferences where
-  "eq_factoring_inferences \<equiv> 
-    { Infer [premise] conclusion | premise conclusion. eq_factoring premise conclusion }"
+  "eq_factoring_inferences \<equiv> { Infer [D] C | D C. eq_factoring D C }"
 
 abbreviation eq_resolution_inferences where
-  "eq_resolution_inferences \<equiv> 
-    { Infer [premise] conclusion | premise conclusion. eq_resolution premise conclusion }"
+  "eq_resolution_inferences \<equiv> { Infer [D] C | D C. eq_resolution D C }"
 
 abbreviation superposition_inferences where
-  "superposition_inferences \<equiv> { Infer [premise\<^sub>2, premise\<^sub>1] conclusion 
-    |  premise\<^sub>2 premise\<^sub>1 conclusion. superposition premise\<^sub>2 premise\<^sub>1 conclusion}"
+  "superposition_inferences \<equiv> { Infer [D, E] C |  D E C. superposition D E C}"
 
 definition inferences :: "('f, 'v, 'ty) typed_clause inference set" where
   "inferences \<equiv> superposition_inferences \<union> eq_resolution_inferences \<union> eq_factoring_inferences"
 
+(* TODO: Just name bottom? *)
 abbreviation bottom\<^sub>F :: "('f, 'v, 'ty) typed_clause set" ("\<bottom>\<^sub>F") where
-  "bottom\<^sub>F \<equiv> {({#}, \<V>) | \<V>. all_types \<V> }"
+  "bottom\<^sub>F \<equiv> {({#}, \<V>) | \<V>. infinite_variables_per_type \<V> }"
 
 subsubsection \<open>Alternative Specification of the Superposition Rule\<close>
 
@@ -182,198 +172,152 @@ inductive pos_superposition ::
   "('f, 'v, 'ty) typed_clause \<Rightarrow> ('f, 'v, 'ty) typed_clause \<Rightarrow> ('f, 'v, 'ty) typed_clause \<Rightarrow> bool"
 where
   pos_superpositionI: "
-    term_subst.is_renaming \<rho>\<^sub>1 \<Longrightarrow>
-    term_subst.is_renaming \<rho>\<^sub>2 \<Longrightarrow>
-    clause.vars (P\<^sub>1 \<cdot> \<rho>\<^sub>1) \<inter> clause.vars (P\<^sub>2 \<cdot> \<rho>\<^sub>2) = {} \<Longrightarrow>
-    P\<^sub>1 = add_mset L\<^sub>1 P\<^sub>1' \<Longrightarrow>
-    P\<^sub>2 = add_mset L\<^sub>2 P\<^sub>2' \<Longrightarrow>
-    L\<^sub>1 = s\<^sub>1\<langle>u\<^sub>1\<rangle> \<approx> s\<^sub>1' \<Longrightarrow>
-    L\<^sub>2 = t\<^sub>2 \<approx> t\<^sub>2' \<Longrightarrow>
-    \<not> is_Var u\<^sub>1 \<Longrightarrow>
-    term_subst.is_imgu \<mu> {{u\<^sub>1 \<cdot>t \<rho>\<^sub>1, t\<^sub>2 \<cdot>t \<rho>\<^sub>2}} \<Longrightarrow>
-    welltyped_imgu \<V>\<^sub>3 (u\<^sub>1 \<cdot>t \<rho>\<^sub>1) (t\<^sub>2 \<cdot>t \<rho>\<^sub>2) \<mu> \<Longrightarrow>
-    \<forall>x \<in> clause.vars (P\<^sub>1 \<cdot> \<rho>\<^sub>1). \<V>\<^sub>1 (inv \<rho>\<^sub>1 (Var x)) = \<V>\<^sub>3 x \<Longrightarrow>
-    \<forall>x \<in> clause.vars (P\<^sub>2 \<cdot> \<rho>\<^sub>2). \<V>\<^sub>2 (inv \<rho>\<^sub>2 (Var x)) = \<V>\<^sub>3 x \<Longrightarrow>
-    is_welltyped_on (clause.vars P\<^sub>1) \<V>\<^sub>1 \<rho>\<^sub>1 \<Longrightarrow>
-    is_welltyped_on (clause.vars P\<^sub>2) \<V>\<^sub>2 \<rho>\<^sub>2 \<Longrightarrow>
+    term.is_renaming \<rho>\<^sub>1 \<Longrightarrow>
+    term.is_renaming \<rho>\<^sub>2 \<Longrightarrow>
+    clause.vars (E \<cdot> \<rho>\<^sub>1) \<inter> clause.vars (D \<cdot> \<rho>\<^sub>2) = {} \<Longrightarrow>
+    E = add_mset l\<^sub>1 E' \<Longrightarrow>
+    D = add_mset l\<^sub>2 D' \<Longrightarrow>
+    l\<^sub>1 = c\<^sub>1\<langle>t\<^sub>1\<rangle> \<approx> t\<^sub>1' \<Longrightarrow>
+    l\<^sub>2 = t\<^sub>2 \<approx> t\<^sub>2' \<Longrightarrow>
+    \<not> is_Var t\<^sub>1 \<Longrightarrow>
+    term.is_imgu \<mu> {{t\<^sub>1 \<cdot>t \<rho>\<^sub>1, t\<^sub>2 \<cdot>t \<rho>\<^sub>2}} \<Longrightarrow>
+    welltyped_imgu \<V>\<^sub>3 (t\<^sub>1 \<cdot>t \<rho>\<^sub>1) (t\<^sub>2 \<cdot>t \<rho>\<^sub>2) \<mu> \<Longrightarrow>
+    \<forall>x \<in> clause.vars (E \<cdot> \<rho>\<^sub>1). \<V>\<^sub>1 (inv \<rho>\<^sub>1 (Var x)) = \<V>\<^sub>3 x \<Longrightarrow>
+    \<forall>x \<in> clause.vars (D \<cdot> \<rho>\<^sub>2). \<V>\<^sub>2 (inv \<rho>\<^sub>2 (Var x)) = \<V>\<^sub>3 x \<Longrightarrow>
+    is_welltyped_on (clause.vars E) \<V>\<^sub>1 \<rho>\<^sub>1 \<Longrightarrow>
+    is_welltyped_on (clause.vars D) \<V>\<^sub>2 \<rho>\<^sub>2 \<Longrightarrow>
     (\<And>\<tau> \<tau>'. typed \<V>\<^sub>2 t\<^sub>2 \<tau> \<Longrightarrow> typed \<V>\<^sub>2 t\<^sub>2' \<tau>' \<Longrightarrow> \<tau> = \<tau>') \<Longrightarrow>
-    \<not> (P\<^sub>1 \<cdot> \<rho>\<^sub>1 \<cdot> \<mu> \<preceq>\<^sub>c P\<^sub>2 \<cdot> \<rho>\<^sub>2 \<cdot> \<mu>) \<Longrightarrow>
-    select P\<^sub>1 = {#} \<Longrightarrow>
-    is_strictly_maximal (L\<^sub>1 \<cdot>l \<rho>\<^sub>1 \<cdot>l \<mu>) (P\<^sub>1 \<cdot> \<rho>\<^sub>1 \<cdot> \<mu>) \<Longrightarrow>
-    select P\<^sub>2 = {#} \<Longrightarrow>
-    is_strictly_maximal (L\<^sub>2 \<cdot>l \<rho>\<^sub>2 \<cdot>l \<mu>) (P\<^sub>2 \<cdot> \<rho>\<^sub>2 \<cdot> \<mu>) \<Longrightarrow>
-    \<not> (s\<^sub>1\<langle>u\<^sub>1\<rangle> \<cdot>t \<rho>\<^sub>1 \<cdot>t \<mu> \<preceq>\<^sub>t s\<^sub>1' \<cdot>t \<rho>\<^sub>1 \<cdot>t \<mu>) \<Longrightarrow>
+    \<not> (E \<cdot> \<rho>\<^sub>1 \<cdot> \<mu> \<preceq>\<^sub>c D \<cdot> \<rho>\<^sub>2 \<cdot> \<mu>) \<Longrightarrow>
+    select E = {#} \<Longrightarrow>
+    is_strictly_maximal (l\<^sub>1 \<cdot>l \<rho>\<^sub>1 \<cdot>l \<mu>) (E \<cdot> \<rho>\<^sub>1 \<cdot> \<mu>) \<Longrightarrow>
+    select D = {#} \<Longrightarrow>
+    is_strictly_maximal (l\<^sub>2 \<cdot>l \<rho>\<^sub>2 \<cdot>l \<mu>) (D \<cdot> \<rho>\<^sub>2 \<cdot> \<mu>) \<Longrightarrow>
+    \<not> (c\<^sub>1\<langle>t\<^sub>1\<rangle> \<cdot>t \<rho>\<^sub>1 \<cdot>t \<mu> \<preceq>\<^sub>t t\<^sub>1' \<cdot>t \<rho>\<^sub>1 \<cdot>t \<mu>) \<Longrightarrow>
     \<not> (t\<^sub>2 \<cdot>t \<rho>\<^sub>2 \<cdot>t \<mu> \<preceq>\<^sub>t t\<^sub>2' \<cdot>t \<rho>\<^sub>2 \<cdot>t \<mu>) \<Longrightarrow>
-    C = add_mset ((s\<^sub>1 \<cdot>t\<^sub>c \<rho>\<^sub>1)\<langle>t\<^sub>2' \<cdot>t \<rho>\<^sub>2\<rangle> \<approx> (s\<^sub>1' \<cdot>t \<rho>\<^sub>1)) (P\<^sub>1' \<cdot> \<rho>\<^sub>1 + P\<^sub>2' \<cdot> \<rho>\<^sub>2) \<cdot> \<mu> \<Longrightarrow>
-    all_types \<V>\<^sub>1 \<Longrightarrow> all_types \<V>\<^sub>2 \<Longrightarrow>
-    pos_superposition (P\<^sub>2, \<V>\<^sub>2) (P\<^sub>1, \<V>\<^sub>1) (C, \<V>\<^sub>3)"
+    C = add_mset ((c\<^sub>1 \<cdot>t\<^sub>c \<rho>\<^sub>1)\<langle>t\<^sub>2' \<cdot>t \<rho>\<^sub>2\<rangle> \<approx> (t\<^sub>1' \<cdot>t \<rho>\<^sub>1)) (E' \<cdot> \<rho>\<^sub>1 + D' \<cdot> \<rho>\<^sub>2) \<cdot> \<mu> \<Longrightarrow>
+    infinite_variables_per_type \<V>\<^sub>1 \<Longrightarrow> 
+    infinite_variables_per_type \<V>\<^sub>2 \<Longrightarrow>
+    pos_superposition (D, \<V>\<^sub>2) (E, \<V>\<^sub>1) (C, \<V>\<^sub>3)"
 
 lemma superposition_if_pos_superposition:
-  assumes "pos_superposition P\<^sub>2 P\<^sub>1 C"
-  shows "superposition P\<^sub>2 P\<^sub>1 C"
+  assumes "pos_superposition D E C"
+  shows "superposition D E C"
   using assms
 proof (cases rule: pos_superposition.cases)
-  case (pos_superpositionI \<rho>\<^sub>1 \<rho>\<^sub>2 P\<^sub>1 P\<^sub>2 L\<^sub>1 P\<^sub>1' L\<^sub>2 P\<^sub>2' s\<^sub>1 u\<^sub>1 s\<^sub>1' t\<^sub>2 t\<^sub>2' \<mu> \<V>\<^sub>3 \<V>\<^sub>1 \<V>\<^sub>2 C)
+  case (pos_superpositionI \<rho>\<^sub>1 \<rho>\<^sub>2 E D l\<^sub>1 E' l\<^sub>2 D' c\<^sub>1 t\<^sub>1 t\<^sub>1' t\<^sub>2 t\<^sub>2' \<mu> \<V>\<^sub>3 \<V>\<^sub>1 \<V>\<^sub>2 C)
   then show ?thesis
-    using superpositionI[of \<rho>\<^sub>1 \<rho>\<^sub>2 P\<^sub>1 P\<^sub>2 L\<^sub>1 P\<^sub>1']
+    using superpositionI[of \<rho>\<^sub>1 \<rho>\<^sub>2 E D l\<^sub>1 E' l\<^sub>2 D' Pos c\<^sub>1 t\<^sub>1 t\<^sub>1' t\<^sub>2 t\<^sub>2' \<mu> \<V>\<^sub>3 \<V>\<^sub>1 \<V>\<^sub>2 C]
     by blast
 qed
-
-(*lemma term_subst_is_renaming_iff_ex_inj_fun_on_vars:
-  "term_subst.is_renaming \<rho> \<longleftrightarrow> (\<exists>f. inj f \<and> \<rho> = Var \<circ> f)"*)
 
 inductive neg_superposition ::
   "('f, 'v, 'ty) typed_clause \<Rightarrow> ('f, 'v, 'ty) typed_clause \<Rightarrow> ('f, 'v, 'ty) typed_clause \<Rightarrow> bool"
 where
   neg_superpositionI: "
-    term_subst.is_renaming \<rho>\<^sub>1 \<Longrightarrow>
-    term_subst.is_renaming \<rho>\<^sub>2 \<Longrightarrow>
-    clause.vars (P\<^sub>1 \<cdot> \<rho>\<^sub>1) \<inter> clause.vars (P\<^sub>2 \<cdot> \<rho>\<^sub>2) = {} \<Longrightarrow>
-    P\<^sub>1 = add_mset L\<^sub>1 P\<^sub>1' \<Longrightarrow>
-    P\<^sub>2 = add_mset L\<^sub>2 P\<^sub>2' \<Longrightarrow>
-    L\<^sub>1 = s\<^sub>1\<langle>u\<^sub>1\<rangle> !\<approx> s\<^sub>1' \<Longrightarrow>
-    L\<^sub>2 = t\<^sub>2 \<approx> t\<^sub>2' \<Longrightarrow>
-    \<not> is_Var u\<^sub>1 \<Longrightarrow>
-    term_subst.is_imgu \<mu> {{u\<^sub>1 \<cdot>t \<rho>\<^sub>1, t\<^sub>2 \<cdot>t \<rho>\<^sub>2}} \<Longrightarrow>
-    welltyped_imgu \<V>\<^sub>3 (u\<^sub>1 \<cdot>t \<rho>\<^sub>1) (t\<^sub>2 \<cdot>t \<rho>\<^sub>2) \<mu> \<Longrightarrow>
-    \<forall>x \<in> clause.vars (P\<^sub>1 \<cdot> \<rho>\<^sub>1). \<V>\<^sub>1 (inv \<rho>\<^sub>1 (Var x)) = \<V>\<^sub>3 x \<Longrightarrow>
-    \<forall>x \<in> clause.vars (P\<^sub>2 \<cdot> \<rho>\<^sub>2). \<V>\<^sub>2 (inv \<rho>\<^sub>2 (Var x)) = \<V>\<^sub>3 x \<Longrightarrow>
-    is_welltyped_on (clause.vars P\<^sub>1) \<V>\<^sub>1 \<rho>\<^sub>1 \<Longrightarrow>
-    is_welltyped_on (clause.vars P\<^sub>2) \<V>\<^sub>2 \<rho>\<^sub>2 \<Longrightarrow>
+    term.is_renaming \<rho>\<^sub>1 \<Longrightarrow>
+    term.is_renaming \<rho>\<^sub>2 \<Longrightarrow>
+    clause.vars (E \<cdot> \<rho>\<^sub>1) \<inter> clause.vars (D \<cdot> \<rho>\<^sub>2) = {} \<Longrightarrow>
+    E = add_mset l\<^sub>1 E' \<Longrightarrow>
+    D = add_mset l\<^sub>2 D' \<Longrightarrow>
+    l\<^sub>1 = c\<^sub>1\<langle>t\<^sub>1\<rangle> !\<approx> t\<^sub>1' \<Longrightarrow>
+    l\<^sub>2 = t\<^sub>2 \<approx> t\<^sub>2' \<Longrightarrow>
+    \<not> is_Var t\<^sub>1 \<Longrightarrow>
+    term.is_imgu \<mu> {{t\<^sub>1 \<cdot>t \<rho>\<^sub>1, t\<^sub>2 \<cdot>t \<rho>\<^sub>2}} \<Longrightarrow>
+    welltyped_imgu \<V>\<^sub>3 (t\<^sub>1 \<cdot>t \<rho>\<^sub>1) (t\<^sub>2 \<cdot>t \<rho>\<^sub>2) \<mu> \<Longrightarrow>
+    \<forall>x \<in> clause.vars (E \<cdot> \<rho>\<^sub>1). \<V>\<^sub>1 (inv \<rho>\<^sub>1 (Var x)) = \<V>\<^sub>3 x \<Longrightarrow>
+    \<forall>x \<in> clause.vars (D \<cdot> \<rho>\<^sub>2). \<V>\<^sub>2 (inv \<rho>\<^sub>2 (Var x)) = \<V>\<^sub>3 x \<Longrightarrow>
+    is_welltyped_on (clause.vars E) \<V>\<^sub>1 \<rho>\<^sub>1 \<Longrightarrow>
+    is_welltyped_on (clause.vars D) \<V>\<^sub>2 \<rho>\<^sub>2 \<Longrightarrow>
     (\<And>\<tau> \<tau>'. typed \<V>\<^sub>2 t\<^sub>2 \<tau> \<Longrightarrow> typed \<V>\<^sub>2 t\<^sub>2' \<tau>' \<Longrightarrow> \<tau> = \<tau>') \<Longrightarrow>
-    \<not> (P\<^sub>1 \<cdot> \<rho>\<^sub>1 \<cdot> \<mu> \<preceq>\<^sub>c P\<^sub>2 \<cdot> \<rho>\<^sub>2 \<cdot> \<mu>) \<Longrightarrow>
-    select P\<^sub>1 = {#} \<and> 
-      is_maximal (L\<^sub>1 \<cdot>l \<rho>\<^sub>1 \<cdot>l \<mu>) (P\<^sub>1 \<cdot> \<rho>\<^sub>1 \<cdot> \<mu>) \<or> is_maximal (L\<^sub>1 \<cdot>l \<rho>\<^sub>1 \<cdot>l \<mu>) ((select P\<^sub>1) \<cdot> \<rho>\<^sub>1 \<cdot> \<mu>) \<Longrightarrow>
-    select P\<^sub>2 = {#} \<Longrightarrow>
-    is_strictly_maximal (L\<^sub>2 \<cdot>l \<rho>\<^sub>2 \<cdot>l \<mu>) (P\<^sub>2 \<cdot> \<rho>\<^sub>2 \<cdot> \<mu>) \<Longrightarrow>
-    \<not> (s\<^sub>1\<langle>u\<^sub>1\<rangle> \<cdot>t \<rho>\<^sub>1 \<cdot>t \<mu> \<preceq>\<^sub>t s\<^sub>1' \<cdot>t \<rho>\<^sub>1 \<cdot>t \<mu>) \<Longrightarrow>
+    \<not> (E \<cdot> \<rho>\<^sub>1 \<cdot> \<mu> \<preceq>\<^sub>c D \<cdot> \<rho>\<^sub>2 \<cdot> \<mu>) \<Longrightarrow>
+    select E = {#} \<and> 
+      is_maximal (l\<^sub>1 \<cdot>l \<rho>\<^sub>1 \<cdot>l \<mu>) (E \<cdot> \<rho>\<^sub>1 \<cdot> \<mu>) \<or> is_maximal (l\<^sub>1 \<cdot>l \<rho>\<^sub>1 \<cdot>l \<mu>) ((select E) \<cdot> \<rho>\<^sub>1 \<cdot> \<mu>) \<Longrightarrow>
+    select D = {#} \<Longrightarrow>
+    is_strictly_maximal (l\<^sub>2 \<cdot>l \<rho>\<^sub>2 \<cdot>l \<mu>) (D \<cdot> \<rho>\<^sub>2 \<cdot> \<mu>) \<Longrightarrow>
+    \<not> (c\<^sub>1\<langle>t\<^sub>1\<rangle> \<cdot>t \<rho>\<^sub>1 \<cdot>t \<mu> \<preceq>\<^sub>t t\<^sub>1' \<cdot>t \<rho>\<^sub>1 \<cdot>t \<mu>) \<Longrightarrow>
     \<not> (t\<^sub>2 \<cdot>t \<rho>\<^sub>2 \<cdot>t \<mu> \<preceq>\<^sub>t t\<^sub>2' \<cdot>t \<rho>\<^sub>2 \<cdot>t \<mu>) \<Longrightarrow>
-    C = add_mset (Neg (Upair (s\<^sub>1 \<cdot>t\<^sub>c \<rho>\<^sub>1)\<langle>t\<^sub>2' \<cdot>t \<rho>\<^sub>2\<rangle>  (s\<^sub>1' \<cdot>t \<rho>\<^sub>1))) (P\<^sub>1' \<cdot> \<rho>\<^sub>1 + P\<^sub>2' \<cdot> \<rho>\<^sub>2) \<cdot> \<mu> \<Longrightarrow>
-    all_types \<V>\<^sub>1 \<Longrightarrow> all_types \<V>\<^sub>2 \<Longrightarrow>
-    neg_superposition (P\<^sub>2, \<V>\<^sub>2) (P\<^sub>1, \<V>\<^sub>1) (C, \<V>\<^sub>3)"
+    C = add_mset ((c\<^sub>1 \<cdot>t\<^sub>c \<rho>\<^sub>1)\<langle>t\<^sub>2' \<cdot>t \<rho>\<^sub>2\<rangle> !\<approx> (t\<^sub>1' \<cdot>t \<rho>\<^sub>1)) (E' \<cdot> \<rho>\<^sub>1 + D' \<cdot> \<rho>\<^sub>2) \<cdot> \<mu> \<Longrightarrow>
+    infinite_variables_per_type \<V>\<^sub>1 \<Longrightarrow> 
+    infinite_variables_per_type \<V>\<^sub>2 \<Longrightarrow>
+    neg_superposition (D, \<V>\<^sub>2) (E, \<V>\<^sub>1) (C, \<V>\<^sub>3)"
 
 lemma superposition_if_neg_superposition:
-  assumes "neg_superposition  P\<^sub>2 P\<^sub>1 C"
-  shows "superposition P\<^sub>2 P\<^sub>1 C"
+  assumes "neg_superposition E D C"
+  shows "superposition E D C"
   using assms
-proof (cases P\<^sub>2 P\<^sub>1 C rule: neg_superposition.cases)
-  case (neg_superpositionI \<rho>\<^sub>1 \<rho>\<^sub>2 P\<^sub>1 L\<^sub>1 P\<^sub>1' P\<^sub>2 L\<^sub>2 P\<^sub>2' s\<^sub>1 u\<^sub>1 s\<^sub>1' t\<^sub>2 t\<^sub>2' \<mu> \<V>\<^sub>3 \<V>\<^sub>1 \<V>\<^sub>2 C)
+proof (cases E D C rule: neg_superposition.cases)
+  case (neg_superpositionI \<rho>\<^sub>1 \<rho>\<^sub>2 E D l\<^sub>1 E' l\<^sub>2 D' c\<^sub>1 t\<^sub>1 t\<^sub>1' t\<^sub>2 t\<^sub>2' \<mu> \<V>\<^sub>3 \<V>\<^sub>1 \<V>\<^sub>2 C)
   then show ?thesis
-    using superpositionI[of \<rho>\<^sub>1 \<rho>\<^sub>2 P\<^sub>1 L\<^sub>1 P\<^sub>1' P\<^sub>2 L\<^sub>2 P\<^sub>2']
+    using superpositionI[of \<rho>\<^sub>1 \<rho>\<^sub>2 E D l\<^sub>1 E' l\<^sub>2 D' Neg c\<^sub>1 t\<^sub>1 t\<^sub>1' t\<^sub>2 t\<^sub>2' \<mu> \<V>\<^sub>3 \<V>\<^sub>1 \<V>\<^sub>2 C]
     by blast
 qed
 
 lemma superposition_iff_pos_or_neg:
-  "superposition P\<^sub>2 P\<^sub>1 C \<longleftrightarrow> pos_superposition P\<^sub>2 P\<^sub>1 C \<or> neg_superposition P\<^sub>2  P\<^sub>1 C"
+  "superposition D E C \<longleftrightarrow> pos_superposition D E C \<or> neg_superposition D E C"
 proof (rule iffI)
-  assume "superposition P\<^sub>2 P\<^sub>1 C"
-  thus "pos_superposition  P\<^sub>2 P\<^sub>1 C \<or> neg_superposition P\<^sub>2 P\<^sub>1 C"
-  proof (cases P\<^sub>2 P\<^sub>1 C rule: superposition.cases)
-    case (superpositionI \<rho>\<^sub>1 \<rho>\<^sub>2 premise\<^sub>1 premise\<^sub>2 literal\<^sub>1 premise\<^sub>1' literal\<^sub>2 premise\<^sub>2' \<P> context\<^sub>1 
-          term\<^sub>1 term\<^sub>1' term\<^sub>2 term\<^sub>2' \<mu>)
+  assume "superposition D E C"
+  thus "pos_superposition D E C \<or> neg_superposition D E C"
+  proof (cases D E C rule: superposition.cases)
+    case (superpositionI \<rho>\<^sub>1 \<rho>\<^sub>2 E D l\<^sub>1 E' l\<^sub>2 D' \<P> c\<^sub>1 t\<^sub>1 t\<^sub>1' t\<^sub>2 t\<^sub>2' \<mu> \<V>\<^sub>3 \<V>\<^sub>1 \<V>\<^sub>2 C)
     then show ?thesis
       using
-        pos_superpositionI[of \<rho>\<^sub>1 \<rho>\<^sub>2 premise\<^sub>1 premise\<^sub>2 literal\<^sub>1 premise\<^sub>1' literal\<^sub>2 premise\<^sub>2' context\<^sub>1 
-                              term\<^sub>1 term\<^sub>1' term\<^sub>2 term\<^sub>2' \<mu>]
-        neg_superpositionI[of \<rho>\<^sub>1 \<rho>\<^sub>2 premise\<^sub>1 premise\<^sub>2 literal\<^sub>1 premise\<^sub>1' literal\<^sub>2 premise\<^sub>2' context\<^sub>1 
-                              term\<^sub>1 term\<^sub>1' term\<^sub>2 term\<^sub>2' \<mu>] 
+        pos_superpositionI[of \<rho>\<^sub>1 \<rho>\<^sub>2 E D l\<^sub>1 E' l\<^sub>2 D' c\<^sub>1 t\<^sub>1 t\<^sub>1' t\<^sub>2 t\<^sub>2' \<mu> \<V>\<^sub>3 \<V>\<^sub>1 \<V>\<^sub>2 C]
+        neg_superpositionI[of \<rho>\<^sub>1 \<rho>\<^sub>2 E D l\<^sub>1 E' l\<^sub>2 D' c\<^sub>1 t\<^sub>1 t\<^sub>1' t\<^sub>2 t\<^sub>2' \<mu> \<V>\<^sub>3 \<V>\<^sub>1 \<V>\<^sub>2 C] 
       by blast
   qed
 next
-  assume "pos_superposition P\<^sub>2 P\<^sub>1 C \<or> neg_superposition P\<^sub>2 P\<^sub>1 C"
-  thus "superposition P\<^sub>2 P\<^sub>1 C"
-    using superposition_if_neg_superposition superposition_if_pos_superposition by metis
+  assume "pos_superposition D E C \<or> neg_superposition D E C"
+  thus "superposition D E C"
+    using superposition_if_neg_superposition superposition_if_pos_superposition 
+    by metis
 qed
 
+(* TODO: Move to other file *)
 lemma eq_resolution_preserves_typing:
-  assumes
-    step: "eq_resolution (D, \<V>) (C, \<V>)" and
-    wt_D: "clause.is_welltyped \<V> D"
+  assumes "eq_resolution (D, \<V>) (C, \<V>)"  "clause.is_welltyped \<V> D"
   shows "clause.is_welltyped \<V> C"
-  using step
-proof (cases "(D, \<V>)" "(C, \<V>)" rule: eq_resolution.cases)
-  case (eq_resolutionI literal premise' "term" term' \<mu>)
-  obtain \<tau> where \<tau>:
-    "welltyped \<V> term \<tau>"
-    "welltyped \<V> term' \<tau>"
-    using wt_D
-    unfolding 
-      eq_resolutionI 
-      clause.is_welltyped_add
-    by auto
-
-  then have "clause.is_welltyped \<V> (D \<cdot> \<mu>)"
-    using wt_D eq_resolutionI(4) clause.is_welltyped.subst_stability
-    by (metis UNIV_I)
-    
-  then show ?thesis
-    using clause.is_welltyped_add
-    unfolding eq_resolutionI
-    by auto
-qed
+  using assms
+  by(cases "(D, \<V>)" "(C, \<V>)" rule: eq_resolution.cases) auto
 
 lemma eq_factoring_preserves_typing:
-  assumes
-    step: "eq_factoring (D, \<V>) (C, \<V>)" and
-    wt_D: "clause.is_welltyped \<V> D"
+  assumes "eq_factoring (D, \<V>) (C, \<V>)" "clause.is_welltyped \<V> D"
   shows "clause.is_welltyped \<V> C"
-  using step
-proof (cases "(D, \<V>)" "(C, \<V>)" rule: eq_factoring.cases)
-  case (eq_factoringI literal\<^sub>1 literal\<^sub>2 premise' term\<^sub>1 term\<^sub>1' term\<^sub>2 term\<^sub>2' \<mu>)
+  using assms
+  by (cases "(D, \<V>)" "(C, \<V>)" rule: eq_factoring.cases) fastforce
 
-  have wt_D\<mu>: "clause.is_welltyped \<V> (D \<cdot> \<mu>)"
-    using wt_D clause.is_welltyped.subst_stability eq_factoringI
-    by (metis UNIV_I)
-
-  show ?thesis
-  proof-
-    (* TODO;: *)
-    show ?thesis
-      using wt_D\<mu>
-      unfolding eq_factoringI
-      apply auto
-       apply (metis literal.sel(1) literal_is_welltyped_iff eq_factoringI(7) subst_atom subst_literal(3) term_subst.is_imgu_unifies')
-      using eq_factoringI(8) by fastforce
-  qed
-qed
-
-(* TODO: Find out where to do it first *)
-declare Term_Context.ground_vars_term_empty [simp del]
-
-(* TODO: Naming!! *)
 lemma superposition_preserves_typing:
   assumes
-    step: "superposition (D, \<V>\<^sub>2) (C, \<V>\<^sub>1) (E, \<V>\<^sub>3)" and
-    wt_C: "clause.is_welltyped \<V>\<^sub>1 C" and
-    wt_D: "clause.is_welltyped \<V>\<^sub>2 D"
-  shows "clause.is_welltyped \<V>\<^sub>3 E"
-  using step
-proof (cases "(D, \<V>\<^sub>2)" "(C, \<V>\<^sub>1)" "(E, \<V>\<^sub>3)" rule: superposition.cases)
-  case (superpositionI \<rho>\<^sub>1 \<rho>\<^sub>2 literal\<^sub>1 premise\<^sub>1' literal\<^sub>2 premise\<^sub>2' \<P> context\<^sub>1 term\<^sub>1 term\<^sub>1' term\<^sub>2 
-         term\<^sub>2' \<mu>)
+    superposition: "superposition (D, \<V>\<^sub>2) (E, \<V>\<^sub>1) (C, \<V>\<^sub>3)" and
+    D_is_welltyped: "clause.is_welltyped \<V>\<^sub>2 D" and
+    E_is_welltyped: "clause.is_welltyped \<V>\<^sub>1 E"
+  shows "clause.is_welltyped \<V>\<^sub>3 C"
+  using superposition
+proof (cases "(D, \<V>\<^sub>2)" "(E, \<V>\<^sub>1)" "(C, \<V>\<^sub>3)" rule: superposition.cases)
+  case (superpositionI \<rho>\<^sub>1 \<rho>\<^sub>2 l\<^sub>1 E' l\<^sub>2 D' \<P> c\<^sub>1 t\<^sub>1 t\<^sub>1' t\<^sub>2 t\<^sub>2' \<mu>)
 
-  have welltyped_\<mu>: "is_welltyped \<V>\<^sub>3 \<mu>"
-    using superpositionI(11)
+  then have welltyped_\<mu>: "is_welltyped \<V>\<^sub>3 \<mu>"
+    by meson
+
+  have "clause.is_welltyped \<V>\<^sub>3 (E \<cdot> \<rho>\<^sub>1)"
+    using E_is_welltyped clause.is_welltyped.typed_renaming[OF superpositionI(1, 12)]
     by blast
 
-  have "clause.is_welltyped \<V>\<^sub>3 (C \<cdot> \<rho>\<^sub>1)"
-    using wt_C clause.is_welltyped.typed_renaming[OF superpositionI(1, 12)] 
-    by blast
-
-  then have wt_C\<mu>: "clause.is_welltyped \<V>\<^sub>3 (C \<cdot> \<rho>\<^sub>1 \<cdot> \<mu>)"
-    by (metis UNIV_I clause.is_welltyped.subst_stability welltyped_\<mu>)
+  then have E\<mu>_is_welltyped: "clause.is_welltyped \<V>\<^sub>3 (E \<cdot> \<rho>\<^sub>1 \<cdot> \<mu>)"
+    using welltyped_\<mu>
+    by simp
    
   have "clause.is_welltyped \<V>\<^sub>3 (D \<cdot> \<rho>\<^sub>2)"
-    using wt_D  clause.is_welltyped.typed_renaming[OF superpositionI(2, 13)] 
+    using D_is_welltyped clause.is_welltyped.typed_renaming[OF superpositionI(2, 13)] 
     by blast    
 
-  then have wt_D\<mu>: "clause.is_welltyped \<V>\<^sub>3 (D \<cdot> \<rho>\<^sub>2 \<cdot> \<mu>)"
-    by (metis UNIV_I clause.is_welltyped.subst_stability welltyped_\<mu>)
+  then have D\<mu>_is_welltyped: "clause.is_welltyped \<V>\<^sub>3 (D \<cdot> \<rho>\<^sub>2 \<cdot> \<mu>)"
+    using welltyped_\<mu>
+    by simp
 
-  have imgu: "term\<^sub>1 \<cdot>t \<rho>\<^sub>1 \<cdot>t \<mu> = term\<^sub>2 \<cdot>t \<rho>\<^sub>2 \<cdot>t \<mu>"
-    using term_subst.is_imgu_unifies'[OF superpositionI(10)].
+  have imgu: "t\<^sub>1 \<cdot>t \<rho>\<^sub>1 \<cdot>t \<mu> = t\<^sub>2 \<cdot>t \<rho>\<^sub>2 \<cdot>t \<mu>"
+    using term.is_imgu_unifies'[OF superpositionI(10)].
 
-  from literal_cases[OF superpositionI(6)] wt_C\<mu> wt_D\<mu> imgu
+  from literal_cases[OF superpositionI(6)] E\<mu>_is_welltyped D\<mu>_is_welltyped imgu
   show ?thesis
     unfolding superpositionI
     by cases auto
