Superposition_Calculus/Nonground_Typing.thy
@@ -9,6 +9,8 @@ theory Nonground_Typing
     Nonground_Order
 begin
 
+type_synonym ('f, 'v, 'ty) typed_clause = "('f, 'v) atom clause \<times> ('v, 'ty) var_types"
+
 locale nonground_typing_lifting = 
   is_typed: typed_subst_stability_lifting where base_typed = base_typed +
   is_welltyped: typed_subst_stability_lifting where 
@@ -37,16 +39,18 @@ locale nonground_uniform_typing_lifting =
 for base_typed base_welltyped :: "('var, 'ty) var_types \<Rightarrow> 'base \<Rightarrow> 'ty \<Rightarrow> bool"
 
 locale term_based_nonground_typing_lifting =
+  "term": nonground_term +
   nonground_typing_lifting where  
   id_subst = Var and comp_subst = "(\<odot>)" and base_subst = "(\<cdot>t)" and base_vars = term.vars
 
 locale term_based_nonground_uniform_typing_lifting =
+  "term": nonground_term +
   nonground_uniform_typing_lifting where  
   id_subst = Var and comp_subst = "(\<odot>)" and map = map_uprod and to_set = set_uprod and 
   sub_vars = term.vars and sub_subst = "(\<cdot>t)"
 
-locale nonground_typing = 
-  test +
+locale nonground_typing =
+  nonground_clause +
   fixes \<F> :: "('f, 'ty) fun_types"
 begin 
 
@@ -57,13 +61,15 @@ sublocale clause_typing "typed (\<V> :: ('v, 'ty) var_types)" "welltyped \<V>"
   by unfold_locales
 
 sublocale atom: term_based_nonground_uniform_typing_lifting where 
-  base_typed = "typed :: ('v \<Rightarrow> 'ty) \<Rightarrow> ('f, 'v) Term.term \<Rightarrow> 'ty \<Rightarrow> bool" and base_welltyped = welltyped 
+  base_typed = "typed :: ('v \<Rightarrow> 'ty) \<Rightarrow> ('f, 'v) Term.term \<Rightarrow> 'ty \<Rightarrow> bool" and 
+  base_welltyped = welltyped 
   by unfold_locales
 
 sublocale literal: term_based_nonground_typing_lifting where 
-  base_typed = "typed :: ('v \<Rightarrow> 'ty) \<Rightarrow> ('f, 'v) Term.term \<Rightarrow> 'ty \<Rightarrow> bool" and base_welltyped = welltyped and
-  sub_vars = atom.vars and sub_subst = "(\<cdot>a)" and map = map_literal and to_set = set_literal and
-  sub_is_typed = atom.is_typed and sub_is_welltyped = atom.is_welltyped 
+  base_typed = "typed :: ('v \<Rightarrow> 'ty) \<Rightarrow> ('f, 'v) Term.term \<Rightarrow> 'ty \<Rightarrow> bool" and 
+  base_welltyped = welltyped and sub_vars = atom.vars and sub_subst = "(\<cdot>a)" and 
+  map = map_literal and to_set = set_literal and sub_is_typed = atom.is_typed and
+  sub_is_welltyped = atom.is_welltyped 
   by unfold_locales
 
 sublocale clause: term_based_nonground_typing_lifting where 
@@ -72,6 +78,27 @@ sublocale clause: term_based_nonground_typing_lifting where
   sub_is_typed = literal.is_typed and sub_is_welltyped = literal.is_welltyped
   by unfold_locales
 
+definition infinite_variables_per_type where 
+  "infinite_variables_per_type \<V> \<equiv> \<forall>ty. infinite {x. \<V> x = ty}"
+
+lemma exists_infinite_variables_per_type:
+  assumes "|UNIV :: 'ty set| \<le>o |UNIV :: ('v :: infinite) set|"
+  shows "\<exists>\<V> :: ('v :: infinite \<Rightarrow> 'ty). infinite_variables_per_type \<V>"
+  using infinite_domain[OF assms infinite_UNIV]
+  unfolding infinite_variables_per_type_def
+  by argo
+
+(* TODO: term_subst.is_ground_subst \<gamma> \<rightarrow> clause.is_ground (fst clause \<cdot> \<gamma>) *)
+(* TODO: Is clause.is_welltyped \<F> (snd clause) (fst clause) needed? *)
+definition clause_groundings :: "('f, 'v, 'ty) typed_clause \<Rightarrow> 'f ground_atom clause set"   where
+  "clause_groundings C = { clause.to_ground (fst C \<cdot> \<gamma>) | \<gamma>. 
+    term.is_ground_subst \<gamma> \<and> 
+    clause.is_welltyped (snd C) (fst C) \<and> 
+    is_welltyped_on (clause.vars (fst C)) (snd C) \<gamma> \<and> 
+    infinite_variables_per_type (snd C)
+  }"
+
 end
+
 
 end
