Superposition_Calculus/Nonground_Term.thy
@@ -5,9 +5,11 @@ theory Nonground_Term
     Ground_Term_Extra
 begin
 
-(* TODO *)
 no_notation subst_compose (infixl "\<circ>\<^sub>s" 75)
+notation subst_compose (infixl "\<odot>" 75)
+
 no_notation subst_apply_term (infixl "\<cdot>" 67)
+notation subst_apply_term (infixl "\<cdot>t" 67)
 
 text \<open>Prefer @{thm [source] term_subst.subst_id_subst} to @{thm [source] subst_apply_term_empty}.\<close>
 declare subst_apply_term_empty[no_atp]
@@ -16,9 +18,6 @@ section \<open>Nonground Terms and Substitutions\<close>
 
 type_synonym 'f ground_term = "'f gterm"
 
-(* TODO: Already here with t or just from Nonground_Clause on?*)
-notation subst_apply_term (infixl "\<cdot>t" 67)
-notation subst_compose (infixl "\<odot>" 75)
 
 subsection\<open>Unified naming\<close>
 
@@ -42,12 +41,27 @@ abbreviation "from_ground \<equiv> from_ground_def"
 
 end
 
-global_interpretation "term": vars_def where vars_def = vars_term.
-
-global_interpretation "term": grounding_def where 
-  to_ground_def = gterm_of_term and from_ground_def = term_of_gterm .
-
 subsection\<open>Term\<close>
+
+locale nonground_term_properties =
+  base_functional_substitution +
+  finite_variables +
+  all_subst_ident_iff_ground + 
+  renaming_variables +
+  vars_subst
+
+locale term_grounding =
+  variables_in_base_imgu where base_vars = vars and base_subst = subst +
+  grounding
+
+(* TODO: Is there a better way for this? *) 
+locale nonground_term 
+begin
+
+sublocale vars_def where vars_def = vars_term.
+
+sublocale grounding_def where 
+  to_ground_def = gterm_of_term and from_ground_def = term_of_gterm .
 
 lemma infinite_terms [intro]: "infinite (UNIV :: ('f, 'v) term set)"
 proof-
@@ -63,7 +77,7 @@ qed
 
 lemma renaming_vars_term:
   assumes "\<forall>x. is_Var (\<rho> x)"
-  shows "Var ` term.vars (t \<cdot>t \<rho>) = \<rho> ` (term.vars t)" 
+  shows "Var ` vars (t \<cdot>t \<rho>) = \<rho> ` (vars t)" 
 proof(induction t)
   case Var
   with assms show ?case
@@ -74,18 +88,18 @@ next
 
   {
     fix t x
-    assume "t \<in> set terms" "x \<in> term.vars (t \<cdot>t \<rho>)"
+    assume "t \<in> set terms" "x \<in> vars (t \<cdot>t \<rho>)"
 
-    then have "Var x \<in> \<rho> ` \<Union> (term.vars ` set terms)"
+    then have "Var x \<in> \<rho> ` \<Union> (vars ` set terms)"
       using Fun
       by (smt (verit, del_insts) UN_iff image_UN image_eqI)
   }
 
   moreover { 
     fix t x
-    assume "t \<in> set terms" "x \<in> term.vars t"
+    assume "t \<in> set terms" "x \<in> vars t"
 
-    then have "\<rho> x \<in> Var ` (\<Union>t' \<in> set terms. term.vars (t' \<cdot>t \<rho>))"
+    then have "\<rho> x \<in> Var ` (\<Union>t' \<in> set terms. vars (t' \<cdot>t \<rho>))"
       using Fun
       by (smt (verit, del_insts) UN_iff image_UN image_eqI)
   }
@@ -94,38 +108,27 @@ next
     by auto
 qed
 
-locale nonground_term = 
-  base_functional_substitution +
-  finite_variables +
-  all_subst_ident_iff_ground + 
-  renaming_variables +
-  vars_subst
-
-locale term_grounding =
-  variables_in_base_imgu where base_vars = vars and base_subst = subst +
-  grounding
-
-global_interpretation "term": nonground_term where subst = "(\<cdot>t)" and  id_subst = Var and 
-  comp_subst = "(\<odot>)" and
-   vars = "term.vars :: ('f, 'v) term \<Rightarrow> 'v set"  and subst_domain = subst_domain and 
-   range_vars = range_vars
+sublocale nonground_term_properties where 
+  subst = "(\<cdot>t)" and id_subst = Var and comp_subst = "(\<odot>)" and 
+  vars = "vars :: ('f, 'v) term \<Rightarrow> 'v set" and subst_domain = subst_domain and 
+  range_vars = range_vars
 proof unfold_locales
   fix t :: "('f, 'v) term"  and \<sigma> \<tau> :: "('f, 'v) subst"
-  assume "\<And>x. x \<in> term.vars t \<Longrightarrow> \<sigma> x = \<tau> x"
+  assume "\<And>x. x \<in> vars t \<Longrightarrow> \<sigma> x = \<tau> x"
   then show "t \<cdot>t \<sigma> = t \<cdot>t \<tau>"
     by(rule term_subst_eq)
 next
   fix t :: "('f, 'v) term"
-  show "finite (term.vars t)"
+  show "finite (vars t)"
     by simp
 next
   fix t :: "('f, 'v) term"
-  show "(term.vars t = {}) = (\<forall>\<sigma>. t \<cdot>t \<sigma> = t)"
+  show "(vars t = {}) = (\<forall>\<sigma>. t \<cdot>t \<sigma> = t)"
     using is_ground_trm_iff_ident_forall_subst.
 next
   fix t :: "('f, 'v) term" and ts :: "('f, 'v) term set"
 
-  assume "finite ts" "term.vars t \<noteq> {}"
+  assume "finite ts" "vars t \<noteq> {}"
   then show "\<exists>\<sigma>. t \<cdot>t \<sigma> \<noteq> t \<and> t \<cdot>t \<sigma> \<notin> ts"
   proof(induction t arbitrary: ts)
     case (Var x)
@@ -151,8 +154,9 @@ next
   next
     case (Fun f args)
 
-    obtain a where a: "a \<in> set args" and a_vars: "term.vars a \<noteq> {}"
-      using Fun.prems by fastforce
+    obtain a where a: "a \<in> set args" and a_vars: "vars a \<noteq> {}"
+      using Fun.prems 
+      by fastforce
 
     then obtain \<sigma> where 
       \<sigma>: "a \<cdot>t \<sigma> \<noteq> a" and
@@ -174,23 +178,23 @@ next
 next
   fix t :: "('f, 'v) term" and \<gamma> :: "('f, 'v) subst"
 
-  show "term.vars (t \<cdot>t \<gamma>) = {} \<longleftrightarrow> (\<forall>x \<in> term.vars t. term.vars (\<gamma> x) = {})"
+  show "vars (t \<cdot>t \<gamma>) = {} \<longleftrightarrow> (\<forall>x \<in> vars t. vars (\<gamma> x) = {})"
     using is_ground_iff.
 next
-  show "\<exists>t. term.vars t = {}"
+  show "\<exists>t. vars t = {}"
     using vars_term_of_gterm
     by metis
 next
   fix t :: "('f, 'v) term" and \<rho> :: "('f, 'v) subst"
   assume "term_subst.is_renaming \<rho>"
 
-  then show "Var ` term.vars (t \<cdot>t \<rho>) = \<rho> ` term.vars t"
+  then show "Var ` vars (t \<cdot>t \<rho>) = \<rho> ` vars t"
     unfolding term_subst_is_renaming_iff
     using renaming_vars_term
     by meson
 next
   fix t :: "('f, 'v) term" and \<sigma>
-  show "term.vars (t \<cdot>t \<sigma>) \<subseteq> term.vars t - subst_domain \<sigma> \<union> range_vars \<sigma>"
+  show "vars (t \<cdot>t \<sigma>) \<subseteq> vars t - subst_domain \<sigma> \<union> range_vars \<sigma>"
     by (rule vars_term_subst_apply_term_subset)
 next
   fix \<rho> :: "('f, 'v) subst" and x
@@ -200,12 +204,10 @@ next
     by blast
 qed
 
-hide_fact term.ground_subst_iff_base_ground_subst
-
-
-global_interpretation "term": term_grounding where subst = "(\<cdot>t)" and id_subst = Var and 
-  comp_subst = "(\<odot>)" and vars = "term.vars :: ('f, 'v) term \<Rightarrow> 'v set" and 
-  from_ground = term.from_ground and to_ground = term.to_ground
+sublocale term_grounding where 
+  subst = "(\<cdot>t)" and id_subst = Var and comp_subst = "(\<odot>)" and 
+  vars = "vars :: ('f, 'v) term \<Rightarrow> 'v set" and from_ground = from_ground and 
+  to_ground = to_ground
 proof unfold_locales
    fix t :: "('f, 'v) term" and \<mu>  :: "('f, 'v) subst" and unifications
 
@@ -214,50 +216,53 @@ proof unfold_locales
     "\<forall>unification\<in>unifications. finite unification"
     "finite unifications" 
 
-  show "term.vars (t \<cdot>t \<mu>) \<subseteq> term.vars t \<union> \<Union> (term.vars ` \<Union> unifications)"
+  show "vars (t \<cdot>t \<mu>) \<subseteq> vars t \<union> \<Union> (vars ` \<Union> unifications)"
     using range_vars_subset_if_is_imgu[OF imgu] vars_term_subst_apply_term_subset
     by fastforce
 next
   {
     fix t :: "('f, 'v) term"
-    assume t_is_ground: "term.is_ground t"
+    assume t_is_ground: "is_ground t"
 
-    have "\<exists>g. term.from_ground g = t"
+    have "\<exists>g. from_ground g = t"
     proof(intro exI)
 
       from t_is_ground 
-      show "term.from_ground (term.to_ground t) = t"
+      show "from_ground (to_ground t) = t"
         by(induction t)(simp_all add: map_idI)
 
     qed
   }
 
-  then show "{t :: ('f, 'v) term. term.is_ground t} = range term.from_ground"
+  then show "{t :: ('f, 'v) term. is_ground t} = range from_ground"
     by fastforce
 next
   fix t\<^sub>G :: "('f) ground_term"
-  show "term.to_ground (term.from_ground t\<^sub>G) = t\<^sub>G"
+  show "to_ground (from_ground t\<^sub>G) = t\<^sub>G"
     by simp
 qed
 
-lemma term_context_ground_iff_term_is_ground [simp]: "Term_Context.ground t = term.is_ground t"
+lemma term_context_ground_iff_term_is_ground [simp]: "Term_Context.ground t = is_ground t"
   by(induction t) simp_all
 
 declare Term_Context.ground_vars_term_empty [simp del]
 
 lemma obtain_ground_fun:
-  assumes "term.is_ground t"
+  assumes "is_ground t"
   obtains f ts where "t = Fun f ts"
   using assms
   by(cases t) auto
 
-lemma renaming_surj_the_inv: 
+(* TODO: Move *)
+lemma renaming_surj_inv: 
   fixes \<rho> :: "('f, 'v) subst"
   assumes "term_subst.is_renaming \<rho>"
   shows "surj (\<lambda>x. inv \<rho> (Var x))"
   using assms inv_f_f
   unfolding term_subst_is_renaming_iff is_Var_def surj_def
   by metis
+
+end
 
 subsection\<open>Setup for lifting from terms\<close>
 
@@ -269,7 +274,8 @@ locale lifting =
   variables_in_base_imgu_lifting +
   vars_subst_lifting
 
-locale lifting_from_term =
+locale term_based_lifting =
+  "term": nonground_term +
   lifting where comp_subst = "(\<odot>)" and id_subst = Var and subst_domain = subst_domain and 
   range_vars = range_vars and base_subst = "(\<cdot>t)" and base_vars = term.vars
 
